fairness/examples/ticketlock/ticketlock_model_lm.v
@@ -1,0 +1,112 @@
+From trillium.fairness Require Import fuel. 
+From trillium.fairness.examples.ticketlock Require Import fair_lock ticketlock_model fair_lock_lm. 
+
+Section TlLM.
+  Let M := tl_fair_model.
+  Let G := @FlG M.
+  Let R := fmrole tl_fair_model.
+  
+  Context {n_roles: nat}.
+  Let roles: gset R := dom $ snd $ tl_init_st' n_roles. 
+  Let gs: gset G := set_map asG roles. 
+  
+  Definition LSI_Tl (st: fmstate M) (tm: groups_map) (fm: @fuel_map M) :=
+    (* LSI_groups_fixed gs st tm fm /\ *) (* <- implied by last condition *)
+    forall ρ, default ∅ (tm !! asG ρ) ⊆ {[ ρ ]} /\           
+    (* ¬ is_unused ρ st <-> asG ρ ∈ dom tm.  *)
+    dom tm = gs. 
+
+  Definition tl_fl := 100. 
+  
+  Definition tl_model: LiveModel G M LSI_Tl :=
+    {| lm_fl _ := tl_fl; |}.
+
+  Instance tl_step_dec s1 ρ s2: Decision (fmtrans M s1 (Some ρ) s2).
+  Proof.
+    Local Ltac nostep := right; intros S; inversion S; subst; set_solver.
+    destruct s1 as [o1 t1 rm1 wf1], s2 as [o2 t2 rm2 wf2].
+    destruct (rm1 !! ρ) as [[s e]| ] eqn:RR.
+    2: { nostep. }
+    destruct e.
+    2: { nostep. } 
+    destruct s as [| k]. 
+    { destruct (decide (
+                      o2 = o1 /\ t2 = t1 + 1 /\ 
+                      let next_en := if decide (o1 = t1) then false else true in
+                      rm2 = <[ρ := (tl_U t1, next_en)]> rm1)) as [T| ?].
+      - destruct T as (->&->&->).
+        left. by constructor.
+      - nostep. }
+    destruct (decide (o1 ≠ k /\ o2 = o1 /\ t2 = t1 /\ rm2 = rm1)) as [T| ?].
+    { inversion T as (?&->&->&->). left. by econstructor. }
+    destruct (decide (k = o1 /\
+                        let st' := (o1 + 1, t1, <[ρ := (tl_L, false)]> rm1) in
+                        let st'' := advance_next st' in
+                        (o2, t2, rm2) = st'')) as [T |]. 
+    { destruct T as [-> ST2].
+      left. simpl. red. simpl.
+      rewrite ST2. by econstructor. }
+    nostep.
+  Qed.
+
+(*   (* TODO: move, upstream *) *)
+(*   Lemma dom_set_to_map: *)
+(* (* B is element type, C is container, K is key, A is value, M is map *) *)
+(* ∀ {B C : Type} `{Elements B C} {K A M : Type} `{Insert K A M} `{Empty M} *)
+(*   `{Dom M C}, *)
+(*   forall f X, dom (set_to_map f X) = set_map (fst ∘ f) X. *)
+  Lemma dom_set_to_map_gset_gmap {B K A: Type} `{Countable B} `{Countable K}
+    (f: B -> K * A)
+    (X: gset B): 
+    dom ((set_to_map f X): gmap K A) = set_map (fst ∘ f) X.
+  Proof.
+    simpl. rewrite /set_to_map.
+    rewrite dom_list_to_map_L. set_solver.
+  Qed. 
+
+  Instance tl_inh: Inhabited (lm_ls tl_model).
+  Proof. 
+    apply populate. unshelve refine {|
+        (* ls_under := (tl_init_st', fs_U): fmstate client_model_impl; *)
+        ls_fuel := gset_to_gmap tl_fl roles;
+        ls_tmap := set_to_map (fun ρ => (asG ρ, {[ ρ ]}: gset R)) roles;
+      |}.
+    - esplit. apply (tl_init_st'_wf n_roles).
+    - simpl. rewrite /tl_live_roles. simpl.
+      etrans; [apply dom_filter_subseteq| ].
+      rewrite /roles. simpl.
+      by rewrite !dom_gset_to_gmap.
+    - intros.
+      rewrite !dom_gset_to_gmap.
+      etrans.
+      2: { do 2 (apply exist_proper; intros).
+           rewrite lookup_set_to_map.
+           2: { simpl. congruence. }
+           apply Morphisms_Prop.and_iff_morphism; reflexivity. }
+      simpl. erewrite ex_det_iff2.
+      2: { intros ??  [(?&?&[=]) ?]. subst.
+           apply elem_of_singleton in H3. subst. split; reflexivity. }
+      set_solver. 
+    - red. intros *. rewrite !lookup_set_to_map.
+      2, 3: simpl; congruence.
+      intros ? (?&?&[=]) (?&?&[=]). subst. set_solver.
+    - simpl. repeat split.
+      + simpl. destruct lookup eqn:L; [| done].
+        simpl. eapply @lookup_set_to_map in L.
+        2, 3: apply _.
+        2: set_solver.
+        destruct L as (?&?&[=]). by subst.
+      + rewrite dom_set_to_map_gset_gmap. set_solver.
+  Qed. 
+        
+  Instance TlLF: lm_fair.LMFairPre tl_model.
+  esplit; try by apply _.
+  
+
+End TlLM. 
+
+Section TlFL.
+
+  FL_LM
+
+End TlFL. 
